Wavelet/Semantics/Confluence.lean
@@ -20,14 +20,6 @@ def Lts.StronglyConfluentAt
       lts.Step c₁ l₂ c' ∧
       lts.Step c₂ l₁ c'
 
-/-- Strong confluence of an LTS when restricted to a subset of states. -/
-def Lts.StronglyConfluent
-  {C : Type u} {E : Type v}
-  (lts : Lts C E)
-  (States : C → Prop)
-  (Compat : E → E → Prop) : Prop :=
-  ∀ {c : C}, States c → lts.StronglyConfluentAt Compat c
-
 /-- Similar to `StronglyConfluentAt`, but modulo an equivalence relation on states. -/
 def Lts.StronglyConfluentAtMod
   {C : Type u} {E : Type v}
@@ -45,5 +37,13 @@ def Lts.StronglyConfluentAtMod
       lts.Step c₁ l₂ c₁' ∧
       lts.Step c₂ l₁ c₂' ∧
       Eq c₁' c₂'
+
+/-- Strong confluence of an LTS when restricted to a subset of states. -/
+def Lts.StronglyConfluent
+  {C : Type u} {E : Type v}
+  (lts : Lts C E)
+  (States : C → Prop)
+  (Compat : E → E → Prop) : Prop :=
+  ∀ {c : C}, States c → lts.StronglyConfluentAt Compat c
 
 end Wavelet.Semantics
